Abstract_Substitution: Rework functional substitutions to substitutions and resolve TODOs

thys/Typed_Ordered_Resolution/Ordered_Resolution.thy
@@ -11,8 +11,11 @@ begin
 
 locale ordered_resolution_calculus =
   witnessed_nonground_typing where
-  welltyped = welltyped and term_to_ground = "term_to_ground :: 't \<Rightarrow> 't\<^sub>G" +
+  welltyped = welltyped and term_to_ground = "term_to_ground :: 't \<Rightarrow> 't\<^sub>G" and
+  id_subst = "id_subst :: 'subst" +
+
   nonground_order where less\<^sub>t = less\<^sub>t +
+
   nonground_selection_function where
   select = select and atom_subst = "(\<cdot>t)" and atom_vars = term.vars and
   atom_from_ground = term.from_ground and atom_to_ground = term.to_ground +
@@ -24,54 +27,53 @@ for
   welltyped :: "('v :: infinite, 'ty) var_types \<Rightarrow> 't \<Rightarrow> 'ty \<Rightarrow> bool"
 begin
 
-(* TODO: Names of Clauses *)
-inductive factoring :: "('t, 'v, 'ty) typed_clause \<Rightarrow> ('t, 'v, 'ty) typed_clause \<Rightarrow> bool"
-where
+inductive factoring :: "('t, 'v, 'ty) typed_clause \<Rightarrow> ('t, 'v, 'ty) typed_clause \<Rightarrow> bool" where
   factoringI: 
-  "C = add_mset L\<^sub>1 (add_mset L\<^sub>2 C') \<Longrightarrow>
-  L\<^sub>1 = (Pos t\<^sub>1) \<Longrightarrow>
-  L\<^sub>2 = (Pos t\<^sub>2) \<Longrightarrow>
-  D = (add_mset L\<^sub>1 C') \<cdot> \<mu> \<Longrightarrow>
-  factoring (\<V>, C) (\<V>, D)"
+  "D = add_mset l\<^sub>1 (add_mset l\<^sub>2 D') \<Longrightarrow>
+   l\<^sub>1 = Pos t\<^sub>1 \<Longrightarrow>
+   l\<^sub>2 = Pos t\<^sub>2 \<Longrightarrow>
+   C = (add_mset l\<^sub>1 D') \<cdot> \<mu> \<Longrightarrow>
+   factoring (\<V>, D) (\<V>, C)"
 if
-  "select C = {#}"
-  "is_maximal (L\<^sub>1 \<cdot>l \<mu>) (C \<cdot> \<mu>)"
-  "type_preserving_on (clause.vars C) \<V> \<mu>" 
+  "select D = {#}"
+  "is_maximal (l\<^sub>1 \<cdot>l \<mu>) (D \<cdot> \<mu>)"
+  "type_preserving_on (clause.vars D) \<V> \<mu>" 
   "term.is_imgu \<mu> {{t\<^sub>1, t\<^sub>2}}"
 
 inductive resolution ::
-  "('t, 'v, 'ty) typed_clause \<Rightarrow> ('t, 'v, 'ty) typed_clause \<Rightarrow> ('t, 'v, 'ty) typed_clause \<Rightarrow> bool"
-where
+  "('t, 'v, 'ty) typed_clause \<Rightarrow>
+   ('t, 'v, 'ty) typed_clause \<Rightarrow>
+   ('t, 'v, 'ty) typed_clause \<Rightarrow> bool" where
   resolutionI: 
-   "C = add_mset L\<^sub>1 C' \<Longrightarrow>
-    D = add_mset L\<^sub>2 D' \<Longrightarrow>
-    L\<^sub>1 = (Neg t\<^sub>1) \<Longrightarrow>
-    L\<^sub>2 = (Pos t\<^sub>2) \<Longrightarrow>
-    R = (C' \<cdot> \<rho>\<^sub>1 + D' \<cdot> \<rho>\<^sub>2) \<cdot> \<mu> \<Longrightarrow>
-    resolution (\<V>\<^sub>2, D) (\<V>\<^sub>1, C) (\<V>\<^sub>3, R)"
+  "E = add_mset l\<^sub>1 E' \<Longrightarrow>
+   D = add_mset l\<^sub>2 D' \<Longrightarrow>
+   l\<^sub>1 = Neg t\<^sub>1 \<Longrightarrow>
+   l\<^sub>2 = Pos t\<^sub>2 \<Longrightarrow>
+   C = (E' \<cdot> \<rho>\<^sub>1 + D' \<cdot> \<rho>\<^sub>2) \<cdot> \<mu> \<Longrightarrow>
+   resolution (\<V>\<^sub>2, D) (\<V>\<^sub>1, E) (\<V>\<^sub>3, C)"
 if
   "infinite_variables_per_type \<V>\<^sub>1"
   "infinite_variables_per_type \<V>\<^sub>2"
   "term.is_renaming \<rho>\<^sub>1"
   "term.is_renaming \<rho>\<^sub>2"
-  "clause.vars (C \<cdot> \<rho>\<^sub>1) \<inter> clause.vars (D \<cdot> \<rho>\<^sub>2) = {}"
-  "type_preserving_on (clause.vars (C \<cdot> \<rho>\<^sub>1) \<union> clause.vars (D \<cdot> \<rho>\<^sub>2)) \<V>\<^sub>3 \<mu>" 
+  "clause.vars (E \<cdot> \<rho>\<^sub>1) \<inter> clause.vars (D \<cdot> \<rho>\<^sub>2) = {}"
+  "type_preserving_on (clause.vars (E \<cdot> \<rho>\<^sub>1) \<union> clause.vars (D \<cdot> \<rho>\<^sub>2)) \<V>\<^sub>3 \<mu>" 
   "term.is_imgu \<mu> {{t\<^sub>1 \<cdot>t \<rho>\<^sub>1, t\<^sub>2 \<cdot>t \<rho>\<^sub>2}}"
-  "\<not> (C \<cdot> \<rho>\<^sub>1 \<odot> \<mu> \<preceq>\<^sub>c D \<cdot> \<rho>\<^sub>2 \<odot> \<mu>)"
-  "select C = {#} \<Longrightarrow> is_maximal (L\<^sub>1 \<cdot>l \<rho>\<^sub>1 \<odot> \<mu>) (C \<cdot> \<rho>\<^sub>1 \<odot> \<mu>)"
-  "select C \<noteq> {#} \<Longrightarrow> is_maximal (L\<^sub>1 \<cdot>l \<rho>\<^sub>1 \<odot> \<mu>) ((select C) \<cdot> \<rho>\<^sub>1 \<odot> \<mu>)"
+  "\<not> (E \<cdot> \<rho>\<^sub>1 \<odot> \<mu> \<preceq>\<^sub>c D \<cdot> \<rho>\<^sub>2 \<odot> \<mu>)"
+  "select E = {#} \<Longrightarrow> is_maximal (l\<^sub>1 \<cdot>l \<rho>\<^sub>1 \<odot> \<mu>) (E \<cdot> \<rho>\<^sub>1 \<odot> \<mu>)"
+  "select E \<noteq> {#} \<Longrightarrow> is_maximal (l\<^sub>1 \<cdot>l \<rho>\<^sub>1 \<odot> \<mu>) ((select E) \<cdot> \<rho>\<^sub>1 \<odot> \<mu>)"
   "select D = {#}"
-  "is_strictly_maximal (L\<^sub>2 \<cdot>l \<rho>\<^sub>2 \<odot> \<mu>) (D \<cdot> \<rho>\<^sub>2 \<odot> \<mu>)"
-  "\<forall>x \<in> clause.vars C. \<V>\<^sub>1 x = \<V>\<^sub>3 (term.rename \<rho>\<^sub>1 x)"
+  "is_strictly_maximal (l\<^sub>2 \<cdot>l \<rho>\<^sub>2 \<odot> \<mu>) (D \<cdot> \<rho>\<^sub>2 \<odot> \<mu>)"
+  "\<forall>x \<in> clause.vars E. \<V>\<^sub>1 x = \<V>\<^sub>3 (term.rename \<rho>\<^sub>1 x)"
   "\<forall>x \<in> clause.vars D. \<V>\<^sub>2 x = \<V>\<^sub>3 (term.rename \<rho>\<^sub>2 x)"
-  "type_preserving_on (clause.vars C) \<V>\<^sub>1 \<rho>\<^sub>1"
+  "type_preserving_on (clause.vars E) \<V>\<^sub>1 \<rho>\<^sub>1"
   "type_preserving_on (clause.vars D) \<V>\<^sub>2 \<rho>\<^sub>2"
 
 abbreviation factoring_inferences where
- "factoring_inferences \<equiv> { Infer [C] D | C D. factoring C D}"
+ "factoring_inferences \<equiv> { Infer [D] C | D C. factoring D C }"
 
 abbreviation resolution_inferences where
- "resolution_inferences \<equiv> { Infer [D, C] R | D C R. resolution D C R}"
+ "resolution_inferences \<equiv> { Infer [D, E] C | D E C. resolution D E C }"
 
 definition inferences :: "('t, 'v, 'ty) typed_clause inference set" where
  "inferences \<equiv> resolution_inferences \<union> factoring_inferences"
