thys/First_Order_Clause/IsaFoR_KBO.thy
@@ -11,7 +11,6 @@ theory IsaFoR_KBO
     IsaFoR_Nonground_Context
     Nonground_Order_With_Equality
 
-    (* TODO: Find out why this needs to be imported here already to have available for KBO *)
     Selection_Function_Select_Max
 begin
 
@@ -126,15 +125,16 @@ end
 subsection\<open>Interpret non-ground order with KBO\<close>
 
 interpretation KBO: context_compatible_nonground_order where
-  less\<^sub>t = "less_kbo :: ('f :: weighted,'v) term \<Rightarrow> ('f,'v) term \<Rightarrow> bool" and
-  comp_subst = "(\<circ>\<^sub>s)" and Var = Var and term_subst = "(\<cdot>)" and term_vars = term.vars and
+  less\<^sub>t = "less_kbo :: ('f :: weighted,'v :: infinite) term \<Rightarrow> ('f,'v) term \<Rightarrow> bool" and
+  comp_subst = "(\<circ>\<^sub>s)" and id_subst = Var and term_subst = "(\<cdot>)" and term_vars = term.vars and
+  subst_updates = subst_updates and apply_subst = apply_subst and subst_update = fun_upd and
   compose_context = "(\<circ>\<^sub>c)" and term_from_ground = term.from_ground and
   term_to_ground = term.to_ground and map_context = map_args_actxt and
   to_ground_context_map = map_args_actxt and from_ground_context_map = map_args_actxt and
   context_to_set = set2_actxt and hole = \<box> and apply_context = ctxt_apply_term and 
   occurences = occurences and ground_hole = \<box> and apply_ground_context = apply_ground_context and
   compose_ground_context = "(\<circ>\<^sub>c)" and ground_context_map = map_args_actxt and
-  ground_context_to_set = set2_actxt 
+  ground_context_to_set = set2_actxt
 proof unfold_locales
    show "transp less_kbo"
     using KBO.S_trans
@@ -151,7 +151,7 @@ next
   show "totalp_on (range term.from_ground) less_kbo"
     using less_kbo_gtotal
     unfolding totalp_on_def Term.ground_vars_term_empty term.is_ground_iff_range_from_ground
-    by blast
+    by (metis term.is_ground_iff_range_from_ground)
 next
   fix
     c :: "('f, 'v) context" and
