thys/Typed_Ordered_Resolution/Ordered_Resolution_Completeness.thy
@@ -15,7 +15,7 @@ lemma factoring_lifting:
   fixes
     D\<^sub>G C\<^sub>G :: "'t\<^sub>G clause" and
     D C :: "'t clause" and
-    \<gamma> :: "'v \<Rightarrow> 't"
+    \<gamma> :: 'subst
   defines
     [simp]: "D\<^sub>G \<equiv> clause.to_ground (D \<cdot> \<gamma>)" and
     [simp]: "C\<^sub>G \<equiv> clause.to_ground (C \<cdot> \<gamma>)"
@@ -33,10 +33,10 @@ lemma factoring_lifting:
     "C' \<cdot> \<gamma> = C \<cdot> \<gamma>"
   using ground_factoring
 proof(cases D\<^sub>G C\<^sub>G rule: ground.factoring.cases)
-  case ground_factoringI: (factoringI L\<^sub>G D\<^sub>G' t\<^sub>G)
+  case ground_factoringI: (factoringI l\<^sub>G D\<^sub>G' t\<^sub>G)
 
   have "D \<noteq> {#}"
-    using ground_factoringI(1)
+    using ground_factoringI(3)
     by auto
 
   then obtain l\<^sub>1 where
@@ -50,18 +50,17 @@ proof(cases D\<^sub>G C\<^sub>G rule: ground.factoring.cases)
     l\<^sub>1_\<gamma>: "l\<^sub>1 \<cdot>l \<gamma> = (Pos (term.from_ground t\<^sub>G))" and
     t\<^sub>1_\<gamma>: "t\<^sub>1 \<cdot>t \<gamma> = term.from_ground t\<^sub>G"
   proof-
-    have "is_maximal (literal.from_ground L\<^sub>G) (D \<cdot> \<gamma>)"
-      using D_grounding ground_factoringI(4)
+    have "is_maximal (literal.from_ground l\<^sub>G) (D \<cdot> \<gamma>)"
+      using D_grounding ground_factoringI(2)
       by auto
 
     then have "l\<^sub>1 \<cdot>l \<gamma> = (Pos (term.from_ground t\<^sub>G))"
-      unfolding ground_factoringI(2)
+      unfolding ground_factoringI(4)
       using unique_maximal_in_ground_clause[OF D_grounding l\<^sub>1_\<gamma>_is_maximal]
       by simp
 
     then show ?thesis
       using that
-      unfolding ground_factoringI(2)
       by (metis Neg_atm_of_iff clause_safe_unfolds(9) literal.collapse(1) literal.sel(1)
           subst_polarity_stable(2))
   qed
@@ -75,13 +74,13 @@ proof(cases D\<^sub>G C\<^sub>G rule: ground.factoring.cases)
       using maximal_in_clause[OF l\<^sub>1_is_maximal]
       by (meson multi_member_split)
 
-    moreover have "D \<cdot> \<gamma> = clause.from_ground (add_mset L\<^sub>G ( add_mset L\<^sub>G D\<^sub>G'))"
-      using ground_factoringI(1) C\<^sub>G_def
+    moreover have "D \<cdot> \<gamma> = clause.from_ground (add_mset l\<^sub>G ( add_mset l\<^sub>G D\<^sub>G'))"
+      using ground_factoringI(3) C\<^sub>G_def
       by (metis D\<^sub>G_def D_grounding clause.to_ground_inverse)
 
-    ultimately have "D'' \<cdot> \<gamma> = add_mset (literal.from_ground L\<^sub>G) (clause.from_ground D\<^sub>G')"
+    ultimately have "D'' \<cdot> \<gamma> = add_mset (literal.from_ground l\<^sub>G) (clause.from_ground D\<^sub>G')"
       using l\<^sub>1_\<gamma>
-      by (simp add: ground_factoringI(2))
+      by (simp add: ground_factoringI(4))
 
     then obtain l\<^sub>2 where "l\<^sub>2 \<cdot>l \<gamma> = Pos (term.from_ground t\<^sub>G)" "l\<^sub>2 \<in># D''"
       unfolding clause.subst_def ground_factoringI
@@ -101,11 +100,10 @@ proof(cases D\<^sub>G C\<^sub>G rule: ground.factoring.cases)
     by (metis clause_safe_unfolds(9) is_pos_def literal.sel(1) subst_polarity_stable(2))
 
   have D'_\<gamma>: "D' \<cdot> \<gamma> = clause.from_ground D\<^sub>G'"
-    using D D_grounding ground_factoringI(1,2,3) l\<^sub>1_\<gamma> l\<^sub>2_\<gamma>
+    using D D_grounding ground_factoringI l\<^sub>1_\<gamma> l\<^sub>2_\<gamma>
     by force
 
-  obtain \<mu> \<sigma> where
-    \<gamma>: "\<gamma> = \<mu> \<odot> \<sigma>" and 
+  obtain \<mu> where
     type_preserving_\<mu>: "type_preserving_on (clause.vars D) \<V> \<mu>" and
     imgu: "term.is_imgu \<mu> {{t\<^sub>1, t\<^sub>2}}"
   proof (rule obtain_type_preserving_on_imgu[OF _ that], intro conjI)
@@ -121,6 +119,10 @@ proof(cases D\<^sub>G C\<^sub>G rule: ground.factoring.cases)
       by auto
   qed
 
+  obtain \<sigma> where \<gamma>: "\<gamma> = \<mu> \<odot> \<sigma>"
+    using term.obtain_imgu_absorption[of \<gamma>, OF _ imgu] t\<^sub>1_\<gamma> t\<^sub>2_\<gamma>
+    by auto
+
   let ?C'' = "add_mset l\<^sub>1 D'"
   let ?C' = "?C'' \<cdot> \<mu>"
 
@@ -131,7 +133,7 @@ proof(cases D\<^sub>G C\<^sub>G rule: ground.factoring.cases)
     proof (rule factoringI; (rule D imgu type_preserving_\<mu> refl \<V>)?)
 
       show "select D = {#}"
-        using ground_factoringI(3) select
+        using ground_factoringI(1) select
         by simp
     next
 
@@ -166,7 +168,7 @@ proof(cases D\<^sub>G C\<^sub>G rule: ground.factoring.cases)
       have "C \<cdot> \<gamma> = clause.from_ground (add_mset (Pos t\<^sub>G) D\<^sub>G')"
         using ground_factoringI(5) clause.to_ground_eq[OF C_grounding clause.ground_is_ground]
         unfolding C\<^sub>G_def
-        by (metis clause.from_ground_inverse ground_factoringI(2))
+        by (metis clause.from_ground_inverse ground_factoringI(4))
 
       also have "... = ?C'' \<cdot> \<gamma>"
         using t\<^sub>1_\<gamma> D'_\<gamma> l\<^sub>1_\<gamma>
@@ -213,110 +215,110 @@ qed
 
 lemma resolution_lifting:
   fixes 
-    C\<^sub>G D\<^sub>G R\<^sub>G :: "'t\<^sub>G clause" and
-    C D R :: "'t clause" and
-    \<gamma> \<rho>\<^sub>1 \<rho>\<^sub>2 :: "'v \<Rightarrow> 't" and
+    E\<^sub>G D\<^sub>G C\<^sub>G :: "'t\<^sub>G clause" and
+    E D C :: "'t clause" and
+    \<gamma> \<rho>\<^sub>1 \<rho>\<^sub>2 :: 'subst and
     \<V>\<^sub>1 \<V>\<^sub>2 :: "('v, 'ty) var_types"
   defines
-    [simp]: "C\<^sub>G \<equiv> clause.to_ground (C \<cdot> \<rho>\<^sub>1 \<odot> \<gamma>)" and
+    [simp]: "E\<^sub>G \<equiv> clause.to_ground (E \<cdot> \<rho>\<^sub>1 \<odot> \<gamma>)" and
     [simp]: "D\<^sub>G \<equiv> clause.to_ground (D \<cdot> \<rho>\<^sub>2 \<odot> \<gamma>)" and
-    [simp]: "R\<^sub>G \<equiv> clause.to_ground (R \<cdot> \<gamma>)" and
-    [simp]: "N\<^sub>G \<equiv> ground_instances \<V>\<^sub>1 C \<union> ground_instances \<V>\<^sub>2 D" and
-    [simp]: "\<iota>\<^sub>G \<equiv> Infer [D\<^sub>G, C\<^sub>G] R\<^sub>G"
+    [simp]: "C\<^sub>G \<equiv> clause.to_ground (C \<cdot> \<gamma>)" and
+    [simp]: "N\<^sub>G \<equiv> ground_instances \<V>\<^sub>1 E \<union> ground_instances \<V>\<^sub>2 D" and
+    [simp]: "\<iota>\<^sub>G \<equiv> Infer [D\<^sub>G, E\<^sub>G] C\<^sub>G"
   assumes
-    ground_resolution: "ground.resolution D\<^sub>G C\<^sub>G R\<^sub>G" and
+    ground_resolution: "ground.resolution D\<^sub>G E\<^sub>G C\<^sub>G" and
     \<rho>\<^sub>1: "term.is_renaming \<rho>\<^sub>1" and
     \<rho>\<^sub>2: "term.is_renaming \<rho>\<^sub>2" and
-    rename_apart: "clause.vars (C \<cdot> \<rho>\<^sub>1) \<inter> clause.vars (D \<cdot> \<rho>\<^sub>2) = {}" and
-    C_grounding: "clause.is_ground (C \<cdot> \<rho>\<^sub>1 \<odot> \<gamma>)" and
+    rename_apart: "clause.vars (E \<cdot> \<rho>\<^sub>1) \<inter> clause.vars (D \<cdot> \<rho>\<^sub>2) = {}" and
+    E_grounding: "clause.is_ground (E \<cdot> \<rho>\<^sub>1 \<odot> \<gamma>)" and
     D_grounding: "clause.is_ground (D \<cdot> \<rho>\<^sub>2 \<odot> \<gamma>)" and
-    R_grounding: "clause.is_ground (R \<cdot> \<gamma>)" and
-    select_from_C: "clause.from_ground (select\<^sub>G C\<^sub>G) = (select C) \<cdot> \<rho>\<^sub>1 \<odot> \<gamma>" and
+    C_grounding: "clause.is_ground (C \<cdot> \<gamma>)" and
+    select_from_E: "clause.from_ground (select\<^sub>G E\<^sub>G) = (select E) \<cdot> \<rho>\<^sub>1 \<odot> \<gamma>" and
     select_from_D: "clause.from_ground (select\<^sub>G D\<^sub>G) = (select D) \<cdot> \<rho>\<^sub>2 \<odot> \<gamma>" and
-    type_preserving_\<rho>\<^sub>1_\<gamma>: "type_preserving_on (clause.vars C) \<V>\<^sub>1 (\<rho>\<^sub>1 \<odot> \<gamma>)" and
+    type_preserving_\<rho>\<^sub>1_\<gamma>: "type_preserving_on (clause.vars E) \<V>\<^sub>1 (\<rho>\<^sub>1 \<odot> \<gamma>)" and
     type_preserving_\<rho>\<^sub>2_\<gamma>: "type_preserving_on (clause.vars D) \<V>\<^sub>2 (\<rho>\<^sub>2 \<odot> \<gamma>)" and
-    type_preserving_\<rho>\<^sub>1: "type_preserving_on (clause.vars C) \<V>\<^sub>1 \<rho>\<^sub>1" and
+    type_preserving_\<rho>\<^sub>1: "type_preserving_on (clause.vars E) \<V>\<^sub>1 \<rho>\<^sub>1" and
     type_preserving_\<rho>\<^sub>2: "type_preserving_on (clause.vars D) \<V>\<^sub>2 \<rho>\<^sub>2" and
     \<V>\<^sub>1: "infinite_variables_per_type \<V>\<^sub>1" and
     \<V>\<^sub>2: "infinite_variables_per_type \<V>\<^sub>2"
-  obtains R' \<V>\<^sub>3
+  obtains C' \<V>\<^sub>3
   where
-    "resolution (\<V>\<^sub>2, D) (\<V>\<^sub>1, C) (\<V>\<^sub>3, R')"
-    "\<iota>\<^sub>G \<in> inference_ground_instances (Infer [(\<V>\<^sub>2, D), (\<V>\<^sub>1, C)] (\<V>\<^sub>3, R'))"
-    "R' \<cdot> \<gamma> = R \<cdot> \<gamma>"
+    "resolution (\<V>\<^sub>2, D) (\<V>\<^sub>1, E) (\<V>\<^sub>3, C')"
+    "\<iota>\<^sub>G \<in> inference_ground_instances (Infer [(\<V>\<^sub>2, D), (\<V>\<^sub>1, E)] (\<V>\<^sub>3, C'))"
+    "C' \<cdot> \<gamma> = C \<cdot> \<gamma>"
   using ground_resolution
-proof(cases D\<^sub>G C\<^sub>G R\<^sub>G rule: ground.resolution.cases)
-  case ground_resolutionI: (resolutionI L\<^sub>G\<^sub>C C\<^sub>G' L\<^sub>G\<^sub>D D\<^sub>G' t\<^sub>G)
+proof(cases D\<^sub>G E\<^sub>G C\<^sub>G rule: ground.resolution.cases)
+  case ground_resolutionI: (resolutionI l\<^sub>G\<^sub>1 l\<^sub>G\<^sub>2 E\<^sub>G' D\<^sub>G' t\<^sub>G)
 
-  have C_\<gamma>: "C \<cdot> \<rho>\<^sub>1 \<odot> \<gamma> = clause.from_ground (add_mset L\<^sub>G\<^sub>C C\<^sub>G')"
-    using ground_resolutionI(1)
-    unfolding C\<^sub>G_def
-    by (metis C_grounding clause.to_ground_inverse)
+  have E_\<gamma>: "E \<cdot> \<rho>\<^sub>1 \<odot> \<gamma> = clause.from_ground (add_mset l\<^sub>G\<^sub>1 E\<^sub>G')"
+    using ground_resolutionI(5)
+    unfolding E\<^sub>G_def
+    by (metis E_grounding clause.to_ground_inverse)
 
-  have D_\<gamma>: "D \<cdot> \<rho>\<^sub>2 \<odot> \<gamma> = clause.from_ground (add_mset L\<^sub>G\<^sub>D  D\<^sub>G')"
-    using ground_resolutionI(2) D\<^sub>G_def
+  have D_\<gamma>: "D \<cdot> \<rho>\<^sub>2 \<odot> \<gamma> = clause.from_ground (add_mset l\<^sub>G\<^sub>2 D\<^sub>G')"
+    using ground_resolutionI(6) D\<^sub>G_def
     by (metis D_grounding clause.to_ground_inverse)
 
-  let ?select\<^sub>G_empty = "select\<^sub>G (clause.to_ground (C \<cdot> \<rho>\<^sub>1 \<odot> \<gamma>)) = {#}"
-  let ?select\<^sub>G_not_empty = "select\<^sub>G (clause.to_ground (C \<cdot> \<rho>\<^sub>1 \<odot> \<gamma>)) \<noteq> {#}"
+  let ?select\<^sub>G_empty = "select\<^sub>G (clause.to_ground (E \<cdot> \<rho>\<^sub>1 \<odot> \<gamma>)) = {#}"
+  let ?select\<^sub>G_not_empty = "select\<^sub>G (clause.to_ground (E \<cdot> \<rho>\<^sub>1 \<odot> \<gamma>)) \<noteq> {#}"
 
-  obtain l\<^sub>C where
-    l\<^sub>C_\<gamma>: "l\<^sub>C \<cdot>l \<rho>\<^sub>1 \<odot> \<gamma> = literal.from_ground L\<^sub>G\<^sub>C" and
-    l\<^sub>C_is_maximal: "?select\<^sub>G_empty \<Longrightarrow> is_maximal l\<^sub>C C" and
-    l\<^sub>C_\<gamma>_is_maximal: "?select\<^sub>G_empty \<Longrightarrow> is_maximal (l\<^sub>C \<cdot>l \<rho>\<^sub>1 \<odot> \<gamma>) (C \<cdot> \<rho>\<^sub>1 \<odot> \<gamma>)" and
-    l\<^sub>C_selected: "?select\<^sub>G_not_empty \<Longrightarrow> is_maximal l\<^sub>C (select C)" and
-    l\<^sub>C_\<gamma>_selected: "?select\<^sub>G_not_empty \<Longrightarrow>is_maximal (l\<^sub>C \<cdot>l \<rho>\<^sub>1 \<odot> \<gamma>) ((select C) \<cdot> \<rho>\<^sub>1 \<odot> \<gamma>)" and   
-    l\<^sub>C_in_C: "l\<^sub>C \<in># C"
+  obtain l\<^sub>1 where
+    l\<^sub>1_\<gamma>: "l\<^sub>1 \<cdot>l \<rho>\<^sub>1 \<odot> \<gamma> = literal.from_ground l\<^sub>G\<^sub>1" and
+    l\<^sub>1_is_maximal: "?select\<^sub>G_empty \<Longrightarrow> is_maximal l\<^sub>1 E" and
+    l\<^sub>1_\<gamma>_is_maximal: "?select\<^sub>G_empty \<Longrightarrow> is_maximal (l\<^sub>1 \<cdot>l \<rho>\<^sub>1 \<odot> \<gamma>) (E \<cdot> \<rho>\<^sub>1 \<odot> \<gamma>)" and
+    l\<^sub>1_selected: "?select\<^sub>G_not_empty \<Longrightarrow> is_maximal l\<^sub>1 (select E)" and
+    l\<^sub>1_\<gamma>_selected: "?select\<^sub>G_not_empty \<Longrightarrow>is_maximal (l\<^sub>1 \<cdot>l \<rho>\<^sub>1 \<odot> \<gamma>) (select E \<cdot> \<rho>\<^sub>1 \<odot> \<gamma>)" and   
+    l\<^sub>1_in_E: "l\<^sub>1 \<in># E"
   proof -
-    have C_not_empty: "C \<noteq> {#}"
-      using ground_resolutionI(1)
+    have E_not_empty: "E \<noteq> {#}"
+      using ground_resolutionI(5)
       by auto
 
     then obtain max_l where
-      "is_maximal max_l C" and
-      is_max_in_C_\<gamma>: "is_maximal (max_l \<cdot>l \<rho>\<^sub>1 \<odot> \<gamma>) (C \<cdot> \<rho>\<^sub>1 \<odot> \<gamma>)"
-      using that C_grounding obtain_maximal_literal C_not_empty
+      "is_maximal max_l E" and
+      is_max_in_E_\<gamma>: "is_maximal (max_l \<cdot>l \<rho>\<^sub>1 \<odot> \<gamma>) (E \<cdot> \<rho>\<^sub>1 \<odot> \<gamma>)"
+      using that E_grounding obtain_maximal_literal E_not_empty
       by blast
 
-    moreover then have "max_l \<in># C" 
+    moreover then have "max_l \<in># E" 
       unfolding is_maximal_def
       by blast
 
-    moreover have "max_l \<cdot>l \<rho>\<^sub>1 \<odot> \<gamma> = literal.from_ground L\<^sub>G\<^sub>C" if ?select\<^sub>G_empty
+    moreover have "max_l \<cdot>l \<rho>\<^sub>1 \<odot> \<gamma> = literal.from_ground l\<^sub>G\<^sub>1" if ?select\<^sub>G_empty
     proof -
-      have "ground_is_maximal L\<^sub>G\<^sub>C C\<^sub>G"
-        using ground_resolutionI(6) that
+      have "ground_is_maximal l\<^sub>G\<^sub>1 E\<^sub>G"
+        using ground_resolutionI(2) that
         unfolding is_maximal_def
         by simp
 
       then show ?thesis
-        using unique_maximal_in_ground_clause[OF C_grounding is_max_in_C_\<gamma>] C_grounding
+        using unique_maximal_in_ground_clause[OF E_grounding is_max_in_E_\<gamma>] E_grounding
         unfolding ground_resolutionI(3)
         by simp
     qed
 
     moreover then obtain selected_l where
-      "is_maximal selected_l (select C)"
-      "is_maximal (selected_l \<cdot>l \<rho>\<^sub>1 \<odot> \<gamma>) ((select C) \<cdot> \<rho>\<^sub>1 \<odot> \<gamma>)"
-      "selected_l \<cdot>l \<rho>\<^sub>1 \<odot> \<gamma> = literal.from_ground L\<^sub>G\<^sub>C"
+      "is_maximal selected_l (select E)"
+      "is_maximal (selected_l \<cdot>l \<rho>\<^sub>1 \<odot> \<gamma>) ((select E) \<cdot> \<rho>\<^sub>1 \<odot> \<gamma>)"
+      "selected_l \<cdot>l \<rho>\<^sub>1 \<odot> \<gamma> = literal.from_ground l\<^sub>G\<^sub>1"
     if ?select\<^sub>G_not_empty
     proof -
 
-      have "is_maximal (literal.from_ground L\<^sub>G\<^sub>C) ((select C) \<cdot> \<rho>\<^sub>1 \<odot> \<gamma>)"
+      have "is_maximal (literal.from_ground l\<^sub>G\<^sub>1) (select E \<cdot> \<rho>\<^sub>1 \<odot> \<gamma>)"
         if ?select\<^sub>G_not_empty
-        using ground_resolutionI(6) that
+        using ground_resolutionI(2) that
         unfolding ground_resolutionI(3)
-        by (metis C\<^sub>G_def select_from_C)
+        by (metis E\<^sub>G_def select_from_E)
 
       then show ?thesis
         using
           that
-          obtain_maximal_literal[OF _ select_ground_subst[OF C_grounding]]
-          unique_maximal_in_ground_clause[OF select_ground_subst[OF C_grounding]]
+          obtain_maximal_literal[OF _ select_ground_subst[OF E_grounding]]
+          unique_maximal_in_ground_clause[OF select_ground_subst[OF E_grounding]]
         by (metis (no_types, lifting) clause.magma_subst_empty(1) is_maximal_not_empty)
     qed
 
-    moreover then have "selected_l \<in># C" if ?select\<^sub>G_not_empty
+    moreover then have "selected_l \<in># E" if ?select\<^sub>G_not_empty
       using that maximal_in_clause mset_subset_eqD select_subset
       by meson
 
@@ -325,26 +327,26 @@ proof(cases D\<^sub>G C\<^sub>G R\<^sub>G rule: ground.resolution.cases)
       by blast
   qed
 
-  obtain C' where C: "C = add_mset l\<^sub>C C'"
-    by (meson l\<^sub>C_in_C multi_member_split)
+  obtain E' where E: "E = add_mset l\<^sub>1 E'"
+    by (meson l\<^sub>1_in_E multi_member_split)
 
-  then have C'_\<gamma>: "C' \<cdot> \<rho>\<^sub>1 \<odot> \<gamma> = clause.from_ground C\<^sub>G'"
-    using l\<^sub>C_\<gamma> C_\<gamma>
+  then have E'_\<gamma>: "E' \<cdot> \<rho>\<^sub>1 \<odot> \<gamma> = clause.from_ground E\<^sub>G'"
+    using l\<^sub>1_\<gamma> E_\<gamma>
     by auto
 
-  obtain t\<^sub>C where 
-    l\<^sub>C: "l\<^sub>C = Neg t\<^sub>C" and
-    t\<^sub>C_\<gamma>: "t\<^sub>C \<cdot>t \<rho>\<^sub>1 \<odot> \<gamma> = term.from_ground t\<^sub>G"
-    using l\<^sub>C_\<gamma> 
+  obtain t\<^sub>1 where 
+    l\<^sub>1: "l\<^sub>1 = Neg t\<^sub>1" and
+    t\<^sub>1_\<gamma>: "t\<^sub>1 \<cdot>t \<rho>\<^sub>1 \<odot> \<gamma> = term.from_ground t\<^sub>G"
+    using l\<^sub>1_\<gamma> 
     by (metis Neg_atm_of_iff literal_from_ground_atom_from_ground(1) clause_safe_unfolds(9)
-        ground_resolutionI(3) literal.sel(2) subst_polarity_stable(2))
+        ground_resolutionI(7) literal.sel(2) subst_polarity_stable(2))
 
-  obtain l\<^sub>D where
-    l\<^sub>D_\<gamma>: "l\<^sub>D \<cdot>l \<rho>\<^sub>2 \<odot> \<gamma> = literal.from_ground L\<^sub>G\<^sub>D" and
-    l\<^sub>D_is_strictly_maximal: "is_strictly_maximal l\<^sub>D D"
+  obtain l\<^sub>2 where
+    l\<^sub>2_\<gamma>: "l\<^sub>2 \<cdot>l \<rho>\<^sub>2 \<odot> \<gamma> = literal.from_ground l\<^sub>G\<^sub>2" and
+    l\<^sub>2_is_strictly_maximal: "is_strictly_maximal l\<^sub>2 D"
   proof-
-    have "is_strictly_maximal (literal.from_ground L\<^sub>G\<^sub>D) (D \<cdot> \<rho>\<^sub>2 \<odot> \<gamma>)"
-      using ground_resolutionI(8) D_grounding
+    have "is_strictly_maximal (literal.from_ground l\<^sub>G\<^sub>2) (D \<cdot> \<rho>\<^sub>2 \<odot> \<gamma>)"
+      using ground_resolutionI(4) D_grounding
       by simp
 
     then show ?thesis
@@ -352,74 +354,77 @@ proof(cases D\<^sub>G C\<^sub>G R\<^sub>G rule: ground.resolution.cases)
       by force
   qed
 
-  then have l\<^sub>D_in_D: "l\<^sub>D \<in># D"
+  then have l\<^sub>2_in_D: "l\<^sub>2 \<in># D"
     using strictly_maximal_in_clause
     by blast
 
-  from l\<^sub>D_\<gamma> have l\<^sub>D_\<gamma>: "l\<^sub>D \<cdot>l \<rho>\<^sub>2 \<odot> \<gamma> = (Pos (term.from_ground t\<^sub>G))"
+  from l\<^sub>2_\<gamma> have l\<^sub>2_\<gamma>: "l\<^sub>2 \<cdot>l \<rho>\<^sub>2 \<odot> \<gamma> = (Pos (term.from_ground t\<^sub>G))"
     unfolding ground_resolutionI
     by simp
 
-  then obtain t\<^sub>D where
-    l\<^sub>D: "l\<^sub>D = Pos t\<^sub>D" and
-    t\<^sub>D_\<gamma>: "t\<^sub>D \<cdot>t \<rho>\<^sub>2 \<odot> \<gamma> = term.from_ground t\<^sub>G"
+  then obtain t\<^sub>2 where
+    l\<^sub>2: "l\<^sub>2 = Pos t\<^sub>2" and
+    t\<^sub>2_\<gamma>: "t\<^sub>2 \<cdot>t \<rho>\<^sub>2 \<odot> \<gamma> = term.from_ground t\<^sub>G"
     by (metis clause_safe_unfolds(9) literal.collapse(1) literal.disc(1) literal.sel(1) 
         subst_polarity_stable(2))
 
-  obtain D' where D: "D = add_mset l\<^sub>D D'"
-    by (meson l\<^sub>D_in_D multi_member_split)
+  obtain D' where D: "D = add_mset l\<^sub>2 D'"
+    by (meson l\<^sub>2_in_D multi_member_split)
 
   then have D'_\<gamma>: "D' \<cdot> \<rho>\<^sub>2 \<odot> \<gamma> = clause.from_ground D\<^sub>G'"
-    using D_\<gamma> l\<^sub>D_\<gamma>
+    using D_\<gamma> l\<^sub>2_\<gamma>
     unfolding ground_resolutionI
     by auto
 
   obtain \<V>\<^sub>3 where
     \<V>\<^sub>3: "infinite_variables_per_type \<V>\<^sub>3" and
-    \<V>\<^sub>1_\<V>\<^sub>3: "\<forall>x\<in>clause.vars C. \<V>\<^sub>1 x = \<V>\<^sub>3 (term.rename \<rho>\<^sub>1 x)" and
+    \<V>\<^sub>1_\<V>\<^sub>3: "\<forall>x\<in>clause.vars E. \<V>\<^sub>1 x = \<V>\<^sub>3 (term.rename \<rho>\<^sub>1 x)" and
     \<V>\<^sub>2_\<V>\<^sub>3: "\<forall>x\<in>clause.vars D. \<V>\<^sub>2 x = \<V>\<^sub>3 (term.rename \<rho>\<^sub>2 x)"
     using clause.obtain_merged_\<V>[OF \<rho>\<^sub>1 \<rho>\<^sub>2 rename_apart clause.finite_vars clause.finite_vars 
         infinite_UNIV] .
 
-  have type_preserving_\<gamma>: "type_preserving_on (clause.vars (C \<cdot> \<rho>\<^sub>1) \<union> clause.vars (D \<cdot> \<rho>\<^sub>2)) \<V>\<^sub>3 \<gamma>"
+  have type_preserving_\<gamma>: "type_preserving_on (clause.vars (E \<cdot> \<rho>\<^sub>1) \<union> clause.vars (D \<cdot> \<rho>\<^sub>2)) \<V>\<^sub>3 \<gamma>"
   proof(unfold Set.ball_Un, intro conjI)
 
-    show "type_preserving_on (clause.vars (C \<cdot> \<rho>\<^sub>1)) \<V>\<^sub>3 \<gamma>"
-      using clause.renaming_grounding[OF \<rho>\<^sub>1 type_preserving_\<rho>\<^sub>1_\<gamma> C_grounding \<V>\<^sub>1_\<V>\<^sub>3] .
+    show "type_preserving_on (clause.vars (E \<cdot> \<rho>\<^sub>1)) \<V>\<^sub>3 \<gamma>"
+      using clause.renaming_grounding[OF \<rho>\<^sub>1 type_preserving_\<rho>\<^sub>1_\<gamma> E_grounding \<V>\<^sub>1_\<V>\<^sub>3] .
   next
 
     show "type_preserving_on (clause.vars (D \<cdot> \<rho>\<^sub>2)) \<V>\<^sub>3 \<gamma>"
       using clause.renaming_grounding[OF \<rho>\<^sub>2 type_preserving_\<rho>\<^sub>2_\<gamma> D_grounding \<V>\<^sub>2_\<V>\<^sub>3] .
   qed
 
-  obtain \<mu> \<sigma> where
-    \<gamma>: "\<gamma> = \<mu> \<odot> \<sigma>" and
-    type_preserving_\<mu>: "type_preserving_on (clause.vars (C \<cdot> \<rho>\<^sub>1) \<union> clause.vars (D \<cdot> \<rho>\<^sub>2)) \<V>\<^sub>3  \<mu>" and
-    imgu: "term.is_imgu \<mu> {{t\<^sub>C \<cdot>t \<rho>\<^sub>1, t\<^sub>D \<cdot>t \<rho>\<^sub>2}}"
+  obtain \<mu> where
+    type_preserving_\<mu>: "type_preserving_on (clause.vars (E \<cdot> \<rho>\<^sub>1) \<union> clause.vars (D \<cdot> \<rho>\<^sub>2)) \<V>\<^sub>3  \<mu>" and
+    imgu: "term.is_imgu \<mu> {{t\<^sub>1 \<cdot>t \<rho>\<^sub>1, t\<^sub>2 \<cdot>t \<rho>\<^sub>2}}"
   proof (rule obtain_type_preserving_on_imgu[OF _ that], intro conjI)
 
-    show "t\<^sub>C \<cdot>t \<rho>\<^sub>1 \<cdot>t \<gamma> = t\<^sub>D \<cdot>t \<rho>\<^sub>2 \<cdot>t \<gamma>"
-      using t\<^sub>C_\<gamma> t\<^sub>D_\<gamma>
+    show "t\<^sub>1 \<cdot>t \<rho>\<^sub>1 \<cdot>t \<gamma> = t\<^sub>2 \<cdot>t \<rho>\<^sub>2 \<cdot>t \<gamma>"
+      using t\<^sub>1_\<gamma> t\<^sub>2_\<gamma>
       by simp
   next
 
-    show "type_preserving_on (term.vars (t\<^sub>C \<cdot>t \<rho>\<^sub>1) \<union> term.vars (t\<^sub>D \<cdot>t \<rho>\<^sub>2)) \<V>\<^sub>3 \<gamma>"
+    show "type_preserving_on (term.vars (t\<^sub>1 \<cdot>t \<rho>\<^sub>1) \<union> term.vars (t\<^sub>2 \<cdot>t \<rho>\<^sub>2)) \<V>\<^sub>3 \<gamma>"
       using type_preserving_\<gamma>
-      unfolding C D l\<^sub>C l\<^sub>D
+      unfolding E D l\<^sub>1 l\<^sub>2
       by auto
   qed
 
-  define R' where
-    R': "R' = (C' \<cdot> \<rho>\<^sub>1 + D' \<cdot> \<rho>\<^sub>2) \<cdot> \<mu>"
+  obtain \<sigma> where \<gamma>: "\<gamma> = \<mu> \<odot> \<sigma>"
+    using term.obtain_imgu_absorption[of \<gamma>, OF _ imgu] t\<^sub>1_\<gamma> t\<^sub>2_\<gamma>
+    by auto
+
+  define C' where
+    C': "C' = (E' \<cdot> \<rho>\<^sub>1 + D' \<cdot> \<rho>\<^sub>2) \<cdot> \<mu>"
 
   show ?thesis
   proof(rule that)
 
-    show resolution: "resolution (\<V>\<^sub>2, D) (\<V>\<^sub>1, C) (\<V>\<^sub>3, R')"
-    proof (rule resolutionI; ((rule \<rho>\<^sub>1 \<rho>\<^sub>2 C D l\<^sub>C l\<^sub>D imgu type_preserving_\<mu> rename_apart 
-            type_preserving_\<rho>\<^sub>1 type_preserving_\<rho>\<^sub>2 \<V>\<^sub>1 \<V>\<^sub>2 R' \<V>\<^sub>1_\<V>\<^sub>3 \<V>\<^sub>2_\<V>\<^sub>3)+)?)
+    show resolution: "resolution (\<V>\<^sub>2, D) (\<V>\<^sub>1, E) (\<V>\<^sub>3, C')"
+    proof (rule resolutionI; ((rule \<rho>\<^sub>1 \<rho>\<^sub>2 E D l\<^sub>1 l\<^sub>2 imgu type_preserving_\<mu> rename_apart 
+            type_preserving_\<rho>\<^sub>1 type_preserving_\<rho>\<^sub>2 \<V>\<^sub>1 \<V>\<^sub>2 C' \<V>\<^sub>1_\<V>\<^sub>3 \<V>\<^sub>2_\<V>\<^sub>3)+)?)
 
-      show "\<not> C \<cdot> \<rho>\<^sub>1 \<odot> \<mu> \<preceq>\<^sub>c D \<cdot> \<rho>\<^sub>2 \<odot> \<mu>"
+      show "\<not> E \<cdot> \<rho>\<^sub>1 \<odot> \<mu> \<preceq>\<^sub>c D \<cdot> \<rho>\<^sub>2 \<odot> \<mu>"
       proof(rule clause.order.ground_less_not_less_eq)
 
         show "clause.vars (D \<cdot> \<rho>\<^sub>2 \<odot> \<mu> \<cdot> \<sigma>) = {}"
@@ -427,72 +432,72 @@ proof(cases D\<^sub>G C\<^sub>G R\<^sub>G rule: ground.resolution.cases)
           unfolding \<gamma>
           by simp
 
-        show "clause.vars (C \<cdot> \<rho>\<^sub>1 \<odot> \<mu> \<cdot> \<sigma>) = {}"
-          using C_grounding
+        show "clause.vars (E \<cdot> \<rho>\<^sub>1 \<odot> \<mu> \<cdot> \<sigma>) = {}"
+          using E_grounding
           unfolding \<gamma>
           by simp
 
-        show "D \<cdot> \<rho>\<^sub>2 \<odot> \<mu> \<cdot> \<sigma> \<prec>\<^sub>c C \<cdot> \<rho>\<^sub>1 \<odot> \<mu> \<cdot> \<sigma>"
-          using ground_resolutionI(5) D_grounding C_grounding
-          unfolding C\<^sub>G_def D\<^sub>G_def clause.order.less\<^sub>G_def \<gamma>
+        show "D \<cdot> \<rho>\<^sub>2 \<odot> \<mu> \<cdot> \<sigma> \<prec>\<^sub>c E \<cdot> \<rho>\<^sub>1 \<odot> \<mu> \<cdot> \<sigma>"
+          using ground_resolutionI(1) D_grounding E_grounding
+          unfolding E\<^sub>G_def D\<^sub>G_def clause.order.less\<^sub>G_def \<gamma>
           by simp
       qed
     next
-      assume "select C = {#}"
+      assume "select E = {#}"
 
       moreover then have ?select\<^sub>G_empty
-        using is_maximal_not_empty l\<^sub>C_selected 
+        using is_maximal_not_empty l\<^sub>1_selected 
         by blast
 
-      moreover have "l\<^sub>C \<cdot>l \<rho>\<^sub>1 \<odot> \<mu> \<in># C \<cdot> \<rho>\<^sub>1 \<odot> \<mu>"
-        using l\<^sub>C_in_C
+      moreover have "l\<^sub>1 \<cdot>l \<rho>\<^sub>1 \<odot> \<mu> \<in># E \<cdot> \<rho>\<^sub>1 \<odot> \<mu>"
+        using l\<^sub>1_in_E
         by blast
 
-      ultimately show "is_maximal (l\<^sub>C \<cdot>l \<rho>\<^sub>1 \<odot> \<mu>) (C \<cdot> \<rho>\<^sub>1 \<odot> \<mu>)"
-        using l\<^sub>C_\<gamma>_is_maximal is_maximal_if_grounding_is_maximal C_grounding 
+      ultimately show "is_maximal (l\<^sub>1 \<cdot>l \<rho>\<^sub>1 \<odot> \<mu>) (E \<cdot> \<rho>\<^sub>1 \<odot> \<mu>)"
+        using l\<^sub>1_\<gamma>_is_maximal is_maximal_if_grounding_is_maximal E_grounding 
         unfolding \<gamma>
         by force
     next
-      assume "select C \<noteq> {#}"
+      assume "select E \<noteq> {#}"
 
       then have "\<not>?select\<^sub>G_empty"
-        using is_maximal_not_empty l\<^sub>C_selected select_from_C 
+        using is_maximal_not_empty l\<^sub>1_selected select_from_E 
         by auto
 
-      moreover have "l\<^sub>C \<cdot>l \<rho>\<^sub>1 \<odot> \<mu> \<in># select C \<cdot> \<rho>\<^sub>1 \<odot> \<mu>"
-        using l\<^sub>C_selected maximal_in_clause calculation 
+      moreover have "l\<^sub>1 \<cdot>l \<rho>\<^sub>1 \<odot> \<mu> \<in># select E \<cdot> \<rho>\<^sub>1 \<odot> \<mu>"
+        using l\<^sub>1_selected maximal_in_clause calculation 
         by blast
 
-      ultimately show "is_maximal (l\<^sub>C \<cdot>l \<rho>\<^sub>1 \<odot> \<mu>) (select C \<cdot> \<rho>\<^sub>1 \<odot> \<mu>)"
-        using select_ground_subst[OF C_grounding] is_maximal_if_grounding_is_maximal l\<^sub>C_\<gamma>_selected
+      ultimately show "is_maximal (l\<^sub>1 \<cdot>l \<rho>\<^sub>1 \<odot> \<mu>) (select E \<cdot> \<rho>\<^sub>1 \<odot> \<mu>)"
+        using select_ground_subst[OF E_grounding] is_maximal_if_grounding_is_maximal l\<^sub>1_\<gamma>_selected
         unfolding \<gamma>
         by fastforce
     next
 
       show "select D = {#}"
-        using ground_resolutionI(7) select_from_D 
+        using ground_resolutionI(3) select_from_D 
         by fastforce
     next
 
-      show "is_strictly_maximal (l\<^sub>D \<cdot>l \<rho>\<^sub>2 \<odot> \<mu>) (D \<cdot> \<rho>\<^sub>2 \<odot> \<mu>)"
+      show "is_strictly_maximal (l\<^sub>2 \<cdot>l \<rho>\<^sub>2 \<odot> \<mu>) (D \<cdot> \<rho>\<^sub>2 \<odot> \<mu>)"
       proof(rule is_strictly_maximal_if_grounding_is_strictly_maximal)
 
-        show "l\<^sub>D \<cdot>l \<rho>\<^sub>2 \<odot> \<mu> \<in># D \<cdot> \<rho>\<^sub>2 \<odot> \<mu>"
-          using l\<^sub>D_in_D
+        show "l\<^sub>2 \<cdot>l \<rho>\<^sub>2 \<odot> \<mu> \<in># D \<cdot> \<rho>\<^sub>2 \<odot> \<mu>"
+          using l\<^sub>2_in_D
           by blast
 
         show "clause.is_ground (D \<cdot> \<rho>\<^sub>2 \<odot> \<mu> \<cdot> \<sigma>)"
           using D_grounding[unfolded \<gamma>]
           by simp
 
-        show "is_strictly_maximal (l\<^sub>D \<cdot>l \<rho>\<^sub>2 \<odot> \<mu> \<cdot>l \<sigma>) (D \<cdot> \<rho>\<^sub>2 \<odot> \<mu> \<cdot> \<sigma>)"
-          using l\<^sub>D_\<gamma> D_\<gamma> ground_resolutionI(8)
+        show "is_strictly_maximal (l\<^sub>2 \<cdot>l \<rho>\<^sub>2 \<odot> \<mu> \<cdot>l \<sigma>) (D \<cdot> \<rho>\<^sub>2 \<odot> \<mu> \<cdot> \<sigma>)"
+          using l\<^sub>2_\<gamma> D_\<gamma> ground_resolutionI(4)
           unfolding \<gamma> ground_resolutionI
           by fastforce
       qed
     qed
 
-    show R'_\<gamma>: "R' \<cdot> \<gamma> = R \<cdot> \<gamma>"
+    show C'_\<gamma>: "C' \<cdot> \<gamma> = C \<cdot> \<gamma>"
     proof-
 
       have "term.is_idem \<mu>"
@@ -503,70 +508,70 @@ proof(cases D\<^sub>G C\<^sub>G R\<^sub>G rule: ground.resolution.cases)
         unfolding \<gamma> term.is_idem_def
         by (metis term.assoc)
 
-      have "R \<cdot> \<gamma> = (clause.from_ground C\<^sub>G' + clause.from_ground D\<^sub>G')"
-        using ground_resolutionI(8, 9) clause.to_ground_inverse[OF R_grounding]
+      have "C \<cdot> \<gamma> = (clause.from_ground E\<^sub>G' + clause.from_ground D\<^sub>G')"
+        using ground_resolutionI(8, 9) clause.to_ground_inverse[OF C_grounding]
         by auto
 
       then show ?thesis
         unfolding
-          R'
-          C'_\<gamma>[symmetric]
+          C'
+          E'_\<gamma>[symmetric]
           D'_\<gamma>[symmetric]
           clause.subst_comp_subst[symmetric]
           \<mu>_\<gamma>
         by simp
     qed
 
-    show "\<iota>\<^sub>G \<in> inference_ground_instances (Infer [(\<V>\<^sub>2, D), (\<V>\<^sub>1, C)] (\<V>\<^sub>3, R'))"
+    show "\<iota>\<^sub>G \<in> inference_ground_instances (Infer [(\<V>\<^sub>2, D), (\<V>\<^sub>1, E)] (\<V>\<^sub>3, C'))"
     proof (rule is_inference_ground_instance_two_premises)
 
-      show "is_inference_ground_instance_two_premises (\<V>\<^sub>2, D) (\<V>\<^sub>1, C) (\<V>\<^sub>3, R') \<iota>\<^sub>G \<gamma> \<rho>\<^sub>1 \<rho>\<^sub>2"
+      show "is_inference_ground_instance_two_premises (\<V>\<^sub>2, D) (\<V>\<^sub>1, E) (\<V>\<^sub>3, C') \<iota>\<^sub>G \<gamma> \<rho>\<^sub>1 \<rho>\<^sub>2"
       proof(unfold split, intro conjI;
           (rule \<rho>\<^sub>1 \<rho>\<^sub>2 rename_apart refl \<V>\<^sub>1 \<V>\<^sub>2 \<V>\<^sub>3)?)
 
-        show "inference.is_ground (Infer [D \<cdot> \<rho>\<^sub>2, C \<cdot> \<rho>\<^sub>1] R' \<cdot>\<iota> \<gamma>)"
-          using  D_grounding C_grounding R_grounding R'_\<gamma>
+        show "inference.is_ground (Infer [D \<cdot> \<rho>\<^sub>2, E \<cdot> \<rho>\<^sub>1] C' \<cdot>\<iota> \<gamma>)"
+          using D_grounding E_grounding C_grounding C'_\<gamma>
           by auto
       next
 
-        show "\<iota>\<^sub>G = inference.to_ground (Infer [D \<cdot> \<rho>\<^sub>2, C \<cdot> \<rho>\<^sub>1] R' \<cdot>\<iota> \<gamma>)"
-          using R'_\<gamma>
+        show "\<iota>\<^sub>G = inference.to_ground (Infer [D \<cdot> \<rho>\<^sub>2, E \<cdot> \<rho>\<^sub>1] C' \<cdot>\<iota> \<gamma>)"
+          using C'_\<gamma>
           by simp
       next
 
-        show "type_preserving_on (clause.vars R') \<V>\<^sub>3 \<gamma>"
+        show "type_preserving_on (clause.vars C') \<V>\<^sub>3 \<gamma>"
         proof(rule type_preserving_on_subset[OF type_preserving_\<gamma>])
 
-          show "clause.vars R' \<subseteq> clause.vars (C \<cdot> \<rho>\<^sub>1) \<union> clause.vars (D \<cdot> \<rho>\<^sub>2)"
+          show "clause.vars C' \<subseteq> clause.vars (E \<cdot> \<rho>\<^sub>1) \<union> clause.vars (D \<cdot> \<rho>\<^sub>2)"
           proof (unfold subset_eq, intro ballI)
             fix x
 
-            have is_imgu: "term.is_imgu \<mu> {{t\<^sub>C \<cdot>t \<rho>\<^sub>1, t\<^sub>D \<cdot>t \<rho>\<^sub>2}}"
+            have is_imgu: "term.is_imgu \<mu> {{t\<^sub>1 \<cdot>t \<rho>\<^sub>1, t\<^sub>2 \<cdot>t \<rho>\<^sub>2}}"
               using imgu
               by blast
 
-            assume "x \<in> clause.vars R'"
+            assume "x \<in> clause.vars C'"
 
             then consider
-              (C') "x \<in> clause.vars (C' \<cdot> \<rho>\<^sub>1 \<odot> \<mu>)" |
+              (E') "x \<in> clause.vars (E' \<cdot> \<rho>\<^sub>1 \<odot> \<mu>)" |
               (D') "x \<in> clause.vars (D' \<cdot> \<rho>\<^sub>2 \<odot> \<mu>)"
-              unfolding R'
+              unfolding C'
               by auto
 
-            then show "x \<in> clause.vars (C \<cdot> \<rho>\<^sub>1) \<union> clause.vars (D \<cdot> \<rho>\<^sub>2)"
+            then show "x \<in> clause.vars (E \<cdot> \<rho>\<^sub>1) \<union> clause.vars (D \<cdot> \<rho>\<^sub>2)"
             proof cases
-              case C'
+              case E'
 
               then show ?thesis
                 using clause.variables_in_base_imgu[OF is_imgu]
-                unfolding C l\<^sub>C D l\<^sub>D
+                unfolding E l\<^sub>1 D l\<^sub>2
                 by auto
             next
               case D'
 
               then show ?thesis
                 using clause.variables_in_base_imgu[OF is_imgu]
-                unfolding C l\<^sub>C D l\<^sub>D
+                unfolding E l\<^sub>1 D l\<^sub>2
                 by auto
             qed
           qed
@@ -661,32 +666,32 @@ lemma resolution_ground_instance:
     "\<iota> \<in> Inf_from N"
     "\<iota>\<^sub>G \<in> inference_ground_instances \<iota>"
 proof-
-  obtain C\<^sub>G D\<^sub>G R\<^sub>G where
-    \<iota>\<^sub>G : "\<iota>\<^sub>G = Infer [D\<^sub>G, C\<^sub>G] R\<^sub>G" and
-    ground_resolution: "ground.resolution D\<^sub>G C\<^sub>G R\<^sub>G"
+  obtain E\<^sub>G D\<^sub>G C\<^sub>G where
+    \<iota>\<^sub>G : "\<iota>\<^sub>G = Infer [D\<^sub>G, E\<^sub>G] C\<^sub>G" and
+    ground_resolution: "ground.resolution D\<^sub>G E\<^sub>G C\<^sub>G"
     using assms(1)
     by blast
 
   have
-    C\<^sub>G_in_groundings: "C\<^sub>G \<in> \<Union> (uncurried_ground_instances ` N)" and
+    E\<^sub>G_in_groundings: "E\<^sub>G \<in> \<Union> (uncurried_ground_instances ` N)" and
     D\<^sub>G_in_groundings: "D\<^sub>G \<in> \<Union> (uncurried_ground_instances ` N)"
     using \<iota>\<^sub>G_Inf_from
     unfolding \<iota>\<^sub>G ground.Inf_from_q_def ground.Inf_from_def
     by simp_all
 
-  obtain C \<V>\<^sub>1 \<gamma>\<^sub>1 where
-    C_grounding: "clause.is_ground (C \<cdot> \<gamma>\<^sub>1)" and
-    type_preserving_\<gamma>\<^sub>1: "type_preserving_on (clause.vars C) \<V>\<^sub>1 \<gamma>\<^sub>1" and
+  obtain E \<V>\<^sub>1 \<gamma>\<^sub>1 where
+    E_grounding: "clause.is_ground (E \<cdot> \<gamma>\<^sub>1)" and
+    type_preserving_\<gamma>\<^sub>1: "type_preserving_on (clause.vars E) \<V>\<^sub>1 \<gamma>\<^sub>1" and
     \<V>\<^sub>1: "infinite_variables_per_type \<V>\<^sub>1" and
-    C_in_N: "(\<V>\<^sub>1, C) \<in> N" and
-    "select\<^sub>G C\<^sub>G = clause.to_ground (select C \<cdot> \<gamma>\<^sub>1)"
-    "C \<cdot> \<gamma>\<^sub>1 = clause.from_ground C\<^sub>G"
-    using subst_stability[rule_format, OF C\<^sub>G_in_groundings]
+    E_in_N: "(\<V>\<^sub>1, E) \<in> N" and
+    "select\<^sub>G E\<^sub>G = clause.to_ground (select E \<cdot> \<gamma>\<^sub>1)"
+    "E \<cdot> \<gamma>\<^sub>1 = clause.from_ground E\<^sub>G"
+    using subst_stability[rule_format, OF E\<^sub>G_in_groundings]
     by blast
 
   then have
-    C\<^sub>G: "C\<^sub>G = clause.to_ground (C \<cdot> \<gamma>\<^sub>1)" and
-    select_from_C: "clause.from_ground (select\<^sub>G C\<^sub>G) = select C \<cdot> \<gamma>\<^sub>1"
+    E\<^sub>G: "E\<^sub>G = clause.to_ground (E \<cdot> \<gamma>\<^sub>1)" and
+    select_from_E: "clause.from_ground (select\<^sub>G E\<^sub>G) = select E \<cdot> \<gamma>\<^sub>1"
     by (simp_all add: select_ground_subst)
 
   obtain D \<V>\<^sub>2 \<gamma>\<^sub>2 where
@@ -704,23 +709,23 @@ proof-
     select_from_D: "clause.from_ground (select\<^sub>G D\<^sub>G) = select D \<cdot> \<gamma>\<^sub>2"
     by (simp_all add: select_ground_subst)
 
-  obtain \<rho>\<^sub>1 \<rho>\<^sub>2 \<gamma> :: "'v \<Rightarrow> 't" where
+  obtain \<rho>\<^sub>1 \<rho>\<^sub>2 \<gamma> where
     \<rho>\<^sub>1: "term.is_renaming \<rho>\<^sub>1" and
     \<rho>\<^sub>2: "term.is_renaming \<rho>\<^sub>2" and
-    rename_apart: "clause.vars (C \<cdot> \<rho>\<^sub>1) \<inter> clause.vars (D \<cdot> \<rho>\<^sub>2) = {}" and
-    type_preserving_\<rho>\<^sub>1: "type_preserving_on (clause.vars C) \<V>\<^sub>1 \<rho>\<^sub>1" and
+    rename_apart: "clause.vars (E \<cdot> \<rho>\<^sub>1) \<inter> clause.vars (D \<cdot> \<rho>\<^sub>2) = {}" and
+    type_preserving_\<rho>\<^sub>1: "type_preserving_on (clause.vars E) \<V>\<^sub>1 \<rho>\<^sub>1" and
     type_preserving_\<rho>\<^sub>2: "type_preserving_on (clause.vars D) \<V>\<^sub>2 \<rho>\<^sub>2" and
-    \<gamma>\<^sub>1_\<gamma>: "\<forall>x \<in> clause.vars C. \<gamma>\<^sub>1 x = (\<rho>\<^sub>1 \<odot> \<gamma>) x" and
-    \<gamma>\<^sub>2_\<gamma>: "\<forall>x \<in> clause.vars D. \<gamma>\<^sub>2 x = (\<rho>\<^sub>2 \<odot> \<gamma>) x"
+    \<gamma>\<^sub>1_\<gamma>: "\<forall>x \<in> clause.vars E. x \<cdot>v \<gamma>\<^sub>1 = x \<cdot>v \<rho>\<^sub>1 \<odot> \<gamma>" and
+    \<gamma>\<^sub>2_\<gamma>: "\<forall>x \<in> clause.vars D. x \<cdot>v \<gamma>\<^sub>2 = x \<cdot>v \<rho>\<^sub>2 \<odot> \<gamma>"
     using clause.obtain_merged_grounding[OF
-        type_preserving_\<gamma>\<^sub>1 type_preserving_\<gamma>\<^sub>2 C_grounding D_grounding \<V>\<^sub>2 clause.finite_vars] .
+        type_preserving_\<gamma>\<^sub>1 type_preserving_\<gamma>\<^sub>2 E_grounding D_grounding \<V>\<^sub>2 clause.finite_vars] .
 
-  have C_grounding: "clause.is_ground (C \<cdot> \<rho>\<^sub>1 \<odot> \<gamma>)"
-    using clause.subst_eq \<gamma>\<^sub>1_\<gamma> C_grounding
+  have E_grounding: "clause.is_ground (E \<cdot> \<rho>\<^sub>1 \<odot> \<gamma>)"
+    using clause.subst_eq \<gamma>\<^sub>1_\<gamma> E_grounding
     by fastforce
 
-  have C\<^sub>G: "C\<^sub>G = clause.to_ground (C \<cdot> \<rho>\<^sub>1 \<odot> \<gamma>)"
-    using clause.subst_eq \<gamma>\<^sub>1_\<gamma> C\<^sub>G
+  have E\<^sub>G: "E\<^sub>G = clause.to_ground (E \<cdot> \<rho>\<^sub>1 \<odot> \<gamma>)"
+    using clause.subst_eq \<gamma>\<^sub>1_\<gamma> E\<^sub>G
     by fastforce
 
   have D_grounding: "clause.is_ground (D \<cdot> \<rho>\<^sub>2 \<odot> \<gamma>)"
@@ -731,7 +736,7 @@ proof-
     using clause.subst_eq \<gamma>\<^sub>2_\<gamma> D\<^sub>G
     by fastforce
 
-  have type_preserving_\<rho>\<^sub>1_\<gamma>: "type_preserving_on (clause.vars C) \<V>\<^sub>1 (\<rho>\<^sub>1 \<odot> \<gamma>)"
+  have type_preserving_\<rho>\<^sub>1_\<gamma>: "type_preserving_on (clause.vars E) \<V>\<^sub>1 (\<rho>\<^sub>1 \<odot> \<gamma>)"
     using type_preserving_\<gamma>\<^sub>1 \<gamma>\<^sub>1_\<gamma>
     by fastforce
 
@@ -739,20 +744,20 @@ proof-
     using type_preserving_\<gamma>\<^sub>2 \<gamma>\<^sub>2_\<gamma>
     by fastforce
 
-  have select_from_C:
-    "clause.from_ground (select\<^sub>G (clause.to_ground (C \<cdot> \<rho>\<^sub>1 \<odot> \<gamma>))) = select C \<cdot> \<rho>\<^sub>1 \<odot> \<gamma>"
+  have select_from_E:
+    "clause.from_ground (select\<^sub>G (clause.to_ground (E \<cdot> \<rho>\<^sub>1 \<odot> \<gamma>))) = select E \<cdot> \<rho>\<^sub>1 \<odot> \<gamma>"
   proof-
-    have "C \<cdot> \<gamma>\<^sub>1 = C \<cdot> \<rho>\<^sub>1 \<odot> \<gamma>"
+    have "E \<cdot> \<gamma>\<^sub>1 = E \<cdot> \<rho>\<^sub>1 \<odot> \<gamma>"
       using \<gamma>\<^sub>1_\<gamma> clause.subst_eq
       by fast
 
-    moreover have "select C \<cdot> \<gamma>\<^sub>1 = select C \<cdot> \<rho>\<^sub>1 \<cdot> \<gamma>"
+    moreover have "select E \<cdot> \<gamma>\<^sub>1 = select E \<cdot> \<rho>\<^sub>1 \<cdot> \<gamma>"
       using clause.subst_eq \<gamma>\<^sub>1_\<gamma> select_vars_subset
       by (metis (no_types, lifting) clause.comp_subst.left.monoid_action_compatibility in_mono)
 
     ultimately show ?thesis
-      using select_from_C
-      unfolding C\<^sub>G
+      using select_from_E
+      unfolding E\<^sub>G
       by simp
   qed
 
@@ -773,36 +778,36 @@ proof-
       by simp
   qed
 
-  obtain R where
-    R_grounding: "clause.is_ground (R \<cdot> \<gamma>)" and
-    R\<^sub>G: "R\<^sub>G = clause.to_ground (R \<cdot> \<gamma>)"
+  obtain C where
+    C_grounding: "clause.is_ground (C \<cdot> \<gamma>)" and
+    C\<^sub>G: "C\<^sub>G = clause.to_ground (C \<cdot> \<gamma>)"
     by (metis clause.all_subst_ident_if_ground clause.from_ground_inverse clause.ground_is_ground)
 
-  have "ground_instances \<V>\<^sub>1 C \<union> ground_instances \<V>\<^sub>2 D \<subseteq> \<Union> (uncurried_ground_instances ` N)"
-    using C_in_N D_in_N
+  have "ground_instances \<V>\<^sub>1 E \<union> ground_instances \<V>\<^sub>2 D \<subseteq> \<Union> (uncurried_ground_instances ` N)"
+    using E_in_N D_in_N
     by force
 
-  obtain R' \<V>\<^sub>3 where
-    resolution: "resolution (\<V>\<^sub>2, D) (\<V>\<^sub>1, C) (\<V>\<^sub>3, R')" and
-    inference_groundings: "\<iota>\<^sub>G \<in> inference_ground_instances (Infer [(\<V>\<^sub>2, D), (\<V>\<^sub>1, C)] (\<V>\<^sub>3, R'))" and
-    R'_\<gamma>_R_\<gamma>: "R' \<cdot> \<gamma> = R \<cdot> \<gamma>"
-    using resolution_lifting[OF ground_resolution[unfolded C\<^sub>G D\<^sub>G R\<^sub>G]
+  obtain C' \<V>\<^sub>3 where
+    resolution: "resolution (\<V>\<^sub>2, D) (\<V>\<^sub>1, E) (\<V>\<^sub>3, C')" and
+    inference_groundings: "\<iota>\<^sub>G \<in> inference_ground_instances (Infer [(\<V>\<^sub>2, D), (\<V>\<^sub>1, E)] (\<V>\<^sub>3, C'))" and
+    C'_\<gamma>_C_\<gamma>: "C' \<cdot> \<gamma> = C \<cdot> \<gamma>"
+    using resolution_lifting[OF ground_resolution[unfolded E\<^sub>G D\<^sub>G C\<^sub>G]
         \<rho>\<^sub>1 \<rho>\<^sub>2
         rename_apart
-        C_grounding D_grounding R_grounding 
-        select_from_C select_from_D
+        E_grounding D_grounding C_grounding 
+        select_from_E select_from_D
         type_preserving_\<rho>\<^sub>1_\<gamma> type_preserving_\<rho>\<^sub>2_\<gamma>
         type_preserving_\<rho>\<^sub>1 type_preserving_\<rho>\<^sub>2
         \<V>\<^sub>1 \<V>\<^sub>2]
-    unfolding \<iota>\<^sub>G R\<^sub>G C\<^sub>G D\<^sub>G .
+    unfolding \<iota>\<^sub>G C\<^sub>G E\<^sub>G D\<^sub>G .
 
-  let ?\<iota> = "Infer [(\<V>\<^sub>2, D), (\<V>\<^sub>1, C)] (\<V>\<^sub>3, R')"
+  let ?\<iota> = "Infer [(\<V>\<^sub>2, D), (\<V>\<^sub>1, E)] (\<V>\<^sub>3, C')"
 
   show ?thesis
   proof(rule that[OF _ inference_groundings])
 
     show "?\<iota> \<in> Inf_from N"
-      using C_in_N D_in_N resolution
+      using E_in_N D_in_N resolution
       unfolding Inf_from_def inferences_def inference_system.Inf_from_def
       by auto
   qed
